\documentclass[a4paper,12pt]{article}
\usepackage[T2A]{fontenc}
\usepackage[utf8]{inputenc}
\usepackage[russian]{babel}
\usepackage{amsmath, amssymb}
\usepackage{setspace}
\usepackage[left=2cm, right=2cm, top=2cm, bottom=2cm]{geometry}


\begin{document}
\setcounter{page}{1}
\setstretch{1.0}
\thispagestyle{empty}
\title{Вариант 12}
\date{}
\maketitle
\section{Задание 4 (испр.). Привести уравнение к каноническому виду и упростить}
Упростим уравнение:
$$2u_{\xi\eta} - u_\eta + 2u = 0$$
Проведем замену:
$$u = e^{\alpha_1\xi + \alpha_2\eta}v$$
$$u_\eta = (\alpha_2 v + v_\eta)e^{\alpha_1\xi + \alpha_2\eta}$$
$$u_{\xi\eta} = (\alpha_2v_\xi + \alpha_1\alpha_2 v + \alpha_1 v_\eta + v_{\xi\eta})e^{\alpha_1\xi + \alpha_2\eta}$$
Вычислим коэффициенты
\begin{align*}
    v_{\xi\eta} &: 2  &v &: 2\alpha_1\alpha_2 - \alpha_2 + 2 \\
    v_\xi &: 2\alpha_2 &v_\eta &: 2\alpha_1 - 1
\end{align*}
Подставим и получим:
$$2v_{\xi\eta} + 2v = 0 \Rightarrow v_{\xi\eta} + v = 0$$
Ответ: $v_{\xi\eta} + v = 0$
\end{document}